Semi-typed formulation is still broken

SemiTyped.v
@@ -4,16 +4,20 @@ Import ListNotations.
 Open Scope list_scope.
 Require Import Program.
 Require Import Contexts.
+Require Import Monad.
 
 
 (* SYNTAX *)
 
 Inductive Pat : WType -> Set :=
 | unit  : Pat One
-| qubit : Pat Qubit
-| bit   : Pat Bit
+| qubit : Var -> Pat Qubit
+| bit   : Var -> Pat Bit
 | pair  : forall {w1 w2}, Pat w1 -> Pat w2 -> Pat (Tensor w1 w2)
 .
+
+
+
 
 Inductive Unitary : WType -> Set := 
   | H : Unitary Qubit 
@@ -41,14 +45,58 @@ Inductive Circuit : WType -> Set :=
 | lift   : forall {w w'}, Pat w -> (interpret w -> Circuit w') -> Circuit w'
 .
 
-Fixpoint compose {W} (c : Circuit W) : forall {W'},
-                             (Pat W -> Circuit W') -> Circuit W' :=
+(*
+
+(* This is a fresh variable monad *)
+Definition Fresh := State nat.
+Definition inc : Fresh () := get >>= fun x => put (S x).
+
+Definition see_var (x : nat) : Fresh () := get >>= fun y => put (max x y).
+Fixpoint see_pat {W} (p : Pat W) : Fresh () :=
+  match p with
+  | unit    => return_ tt
+  | qubit x => see_var x
+  | bit x   => see_var x
+  | pair p1 p2 => see_pat p1 >> see_pat p2
+  end.
+Fixpoint see_circuit {W} (c : Circuit W) : Fresh () :=
   match c with
-  | output p       => fun _ f => f p
-  | gate g p1 p2 k => fun _ f => gate g p1 p2 (compose k f)
-  | lift p g       => fun _ f => lift p (fun p' => compose (g p') f)
+  | output p       => see_pat p
+  | gate g p1 p2 c => see_pat p1 >> see_pat p2 >> see_circuit c
+  | lift p f       => see_pat p (* bad *)
   end.
 
+Fixpoint var {W : WType} : Fresh (Pat W) :=
+  match W with
+  | One => return_ unit
+  | Qubit => inc >> get >>= fun x => return_ (qubit x)
+  | Bit   => inc >> get >>= fun x => return_ (bit x)
+  | Tensor W1 W2 => do p1 ← @var W1;
+                    do p2 ← @var W2;
+                    return_ (pair p1 p2)
+  end.
+
+Definition fresh {W1 W2} (f : Pat W1 -> Circuit W2) : Pat W1 :=
+  runState ( do p0 ← var; 
+             do _  ← see_circuit (f p0);
+             var ) 0.
+
+Definition hoas_gate {W1 W2 W} (g : Gate W1 W2) (p1 : Pat W1) 
+                               (f : Pat W2 -> Circuit W) : Circuit W :=
+  let p2 := fresh f in 
+  gate g p1 p2 (f p2).
+
+ 
+Definition rename {W} {W'} (p' p : Pat W) : Circuit W' -> Circuit W'.
+Admitted.
+*)
+
+Fixpoint compose {W W'} (c : Circuit W) : (Pat W -> Circuit W') -> Circuit W' :=
+  match c with
+  | output p       => fun f => f p
+  | gate g p1 p2 k => fun f => gate g p1 p2 (compose k f)
+  | lift p g       => fun f => lift p (fun p' => compose (g p') f)
+  end.
 
 (* TYPING *) 
 
@@ -56,8 +104,8 @@ Definition Merge (Γ1 Γ2 Γ : Ctx) := Γ1 ⋓ Γ2 = Γ.
 
 Inductive WF_Pat : forall {W}, Ctx -> Pat W -> Set :=
 | wf_unit  : WF_Pat [] unit
-| wf_qubit : forall {x Γ}, SingletonCtx x Qubit Γ -> WF_Pat Γ qubit
-| wf_bit   : forall {x Γ}, SingletonCtx x Bit Γ -> WF_Pat Γ bit
+| wf_qubit : forall {x Γ}, SingletonCtx x Qubit Γ -> WF_Pat Γ (qubit x)
+| wf_bit   : forall {x Γ}, SingletonCtx x Bit Γ -> WF_Pat Γ (bit x)
 | wf_pair  : forall {Γ1 Γ2 Γ : Ctx} {W1 W2} (p1 : Pat W1) (p2 : Pat W2), 
              Merge Γ1 Γ2 Γ ->
              WF_Pat Γ1 p1 -> WF_Pat Γ2 p2 -> WF_Pat Γ (pair p1 p2)
@@ -83,37 +131,88 @@ Inductive WF_Circuit : forall {W}, Ctx -> Circuit W -> Set :=
               WF_Circuit Γ'' (lift p f)
 .
 
+Definition FinMap A := list (option A).
+Fixpoint union {A} (Γ1 Γ2 : FinMap A) : FinMap A :=
+  match Γ1, Γ2 with
+  | [], _ => Γ2
+  | _, [] => Γ1
+  | Some w1 :: Γ1, _  :: Γ2 => Some w1 :: union Γ1 Γ2
+  | None    :: Γ1, w2 :: Γ2 => w2 :: union Γ1 Γ2
+  end.
+
+Fixpoint domain_pat {W} (p : Pat W) : Ctx :=
+  match p with
+  | unit       => []
+  | qubit x    => singleton x W
+  | bit x      => singleton x W
+  | pair p1 p2 => union (domain_pat p1) (domain_pat p2)
+  end.
+
+Fixpoint zip {A B} (ls1 : list A) (ls2 : list B) : list (A * B) :=
+  match ls1, ls2 with
+  | [], _ => []
+  | _, [] => []
+  | a :: ls1, b :: ls2 => (a,b) :: zip ls1 ls2
+  end.
+
+Fixpoint all_vals W : list (interpret W) :=
+  match W with
+  | One     => []
+  | Qubit   => [true;false]
+  | Bit     => [true;false]
+  | W1 ⊗ W2 => zip (all_vals W1) (all_vals W2)
+  end.
+
+Fixpoint domain_circ {W} (c : Circuit W) : Ctx :=
+  match c with
+  | output p       => domain_pat p
+  | gate g p1 p2 c => union (domain_pat p1) (domain_circ c)
+  | lift p f       => 
+    let f' := fun dom x => union dom (domain_circ (f x)) in
+    fold_left f' (all_vals _) (domain_pat p) 
+  end.
 
 
-(* should not be necessary for checking examples *)
+Definition Disjoint (Γ1 Γ2 : OCtx) := {Γ : Ctx & Γ1 ⋓ Γ2 = Valid Γ}.
+Definition Disjoint_Pattern {W} Ω (p : Pat W) : Set := Disjoint Ω (domain_pat p).
+Definition Disjoint_Circuit {W} Ω (c : Circuit W) : Set := Disjoint Ω (domain_circ c).
 
-Lemma wf_compose : forall {W W'} {Γ Γ1 Γ1'} 
+Lemma wf_compose : forall {W W'} {Ω Γ1 Γ1' : Ctx} 
                           (c : Circuit W) (f : Pat W -> Circuit W'),
-      Merge Γ1 Γ Γ1' -> 
-      WF_Circuit Γ1 c -> 
-      (forall (p : Pat W){Γ2 Γ2'}, Merge Γ2 Γ Γ2' -> WF_Pat Γ2 p -> WF_Circuit Γ2' (f p) ) ->
-      WF_Circuit Γ1' (compose c f).
-Admitted.
-(*
+      Disjoint_Circuit Ω c   
+   -> Merge Γ1 Ω Γ1' 
+   -> WF_Circuit Γ1 c
+   -> (forall (p : Pat W){Γ2 Γ2'}, Merge Γ2 Ω Γ2' 
+                                -> WF_Pat Γ2 p -> WF_Circuit Γ2' (f p) )
+   -> WF_Circuit Γ1' (compose c f).
+(*Admitted.*)
 Proof.
-  intros W W' Γ Γ1 Γ1' c f pf_merge wf_c.
-  revert W' Γ Γ1' f pf_merge.
-  induction wf_c; intros W0 Ω Ω1' h pf_merge H; simpl.
+  intros W W' Ω Γ1 Γ1' c f pf_disjoint pf_merge wf_c.
+  revert W' Ω Γ1' f pf_disjoint pf_merge.
+  induction wf_c; intros W0 Ω Ω1' h pf_disjoint pf_merge H; simpl.
   - eapply H; eauto.
-  - econstructor; [ | | eauto | eauto | ].
-    Focus 3. eapply IHwf_c; [ | eauto]. 
-      unfold Merge in *. admit (*?*).
-    * unfold Merge in *. 
-      assert (H0 : Γ1 ⋓ (Γ ⋓ Ω) = Ω1'). admit.
-      destruct (merge_valid _ _ _ H0).  destruct s; destruct s0. 
-      rewrite e0 in H0. exact H0.
-
-rewrite <- pf_merge at (Valid Ω1'). instantiate (0:=Γ ⋓ Ω).
-
-rewrite <- pf_merge at 2.
-
-Ω1' = Γ1' ⋓ Ω = Γ1 ⋓ Γ ⋓ Ω
+  - assert (eq1 : Γ1 ⋓ (Γ ⋓ Ω) = Ω1').
+      { rewrite <- pf_merge. rewrite <- m. rewrite merge_assoc. reflexivity. }
+    remember (Γ ⋓ Ω) as Ω0. destruct Ω0 as [ | Ω0]; [inversion eq1 | ].
+    econstructor; [ | | eauto | eauto | ]; unfold Merge in *.
+    * exact eq1.
     *
-  - 
-  -
-*)
+    *
+    *
+    
+    econstructor; [ | | eauto | eauto | eapply IHwf_c; [ | eauto]];
+    unfold Merge in *; eauto.
+    * rewrite HeqΩ0. rewrite merge_assoc. rewrite m0.
+      
+(* Γ2 ⊥ Γ
+         WTS: Γ2 ⊥ (Γ ⋓ Ω)
+         need: Γ2 ⊥ Ω *)
+      admit.
+    * (* need: Γ2' ⊥ Ω *)
+      admit.
+  - assert (eq1 : Γ ⋓ (Γ' ⋓ Ω) = Ω1'). 
+      { rewrite <- pf_merge. rewrite <- m. rewrite merge_assoc. reflexivity. }
+    remember (Γ' ⋓ Ω) as Ω0. destruct Ω0 as [ | Ω0]; [inversion eq1 | ].
+    econstructor; [ | eauto | intro x; eapply H0; [ | eauto] ];
+    unfold Merge in *; eauto.
+Admitted.
